use trees for quantFree formulas

Quantelim/QuantElim/QuantFreeFormula.lean
@@ -3,43 +3,88 @@ import QuantElim.Poly.Basic
 variable {n : ℕ}
 
 inductive QuantFreeFormula (n : ℕ) : Type
-  | true : QuantFreeFormula n
-  | false : QuantFreeFormula n
-  | neZero : Poly n → QuantFreeFormula n
-  | eqZero : Poly n → QuantFreeFormula n
-  | and : QuantFreeFormula n → QuantFreeFormula n → QuantFreeFormula n
-  | or : QuantFreeFormula n → QuantFreeFormula n → QuantFreeFormula n
+  | tru : QuantFreeFormula n
+  | fals : QuantFreeFormula n
+  | ite' : Poly n → QuantFreeFormula n → QuantFreeFormula n → QuantFreeFormula n
 
 namespace QuantFreeFormula
 
+def rel (p q : Poly n) : Prop :=
+  0 < p.degree ∧ p.degree ≤ q.degree
+
+instance : DecidableRel (@rel n) := fun _ _ => by dsimp [rel]; infer_instance
+
 @[simp]
 def eval : QuantFreeFormula n → Set (Fin n → ℂ)
-  | true => Set.univ
-  | false => ∅
-  | neZero p => { x | p.eval x ≠ 0 }
-  | eqZero p => { x | p.eval x = 0 }
-  | and φ ψ => eval φ ∩ eval ψ
-  | or φ ψ => eval φ ∪ eval ψ
+  | tru => Set.univ
+  | fals => ∅
+  | ite' p φ ψ => ({x | p.eval x = 0} ∩ φ.eval) ∪ ({x | p.eval x ≠ 0} ∩ ψ.eval)
 
 def not : QuantFreeFormula n → QuantFreeFormula n
-  | true => false
-  | false => true
-  | neZero p => eqZero p
-  | eqZero p => neZero p
-  | and φ ψ => or (not φ) (not ψ)
-  | or φ ψ => and (not φ) (not ψ)
+  | tru => fals
+  | fals => tru
+  | ite' p φ ψ => ite' p  (not φ) (not ψ)
 
 @[simp]
 theorem eval_not : ∀ φ : QuantFreeFormula n, eval (not φ) = (eval φ)ᶜ
-  | true => by simp [not, eval]
-  | false => by simp [not, eval]
-  | neZero p => by simp [Set.ext_iff, not, eval, eval_not]
-  | eqZero p => by simp [Set.ext_iff, not, eval, eval_not]
-  | and p q => by simp [Set.ext_iff, not, eval, eval_not]; tauto
-  | or p q => by simp [Set.ext_iff, not, eval, eval_not]
+  | tru => by simp [not, eval]
+  | fals => by simp [not, eval]
+  | ite' p φ ψ => by
+    ext x
+    by_cases h : p.eval x = 0
+    · simp [eval_not, h]
+    · simp [eval_not, h]
+
+def or : ∀ (_φ₁ _φ₂ : QuantFreeFormula n), QuantFreeFormula n
+  | tru, _ => tru
+  | _, tru => tru
+  | fals, φ => φ
+  | φ, fals => φ
+  | ite' p φ ψ, ite' q χ ω =>
+    if rel p q
+    then ite' p (ite' q (φ.or χ) (φ.or ω)) (ite' q (ψ.or χ) (ψ.or ω))
+    else ite' q (ite' p (φ.or χ) (ψ.or χ)) (ite' p (φ.or ω) (ψ.or ω))
+
+@[simp]
+theorem eval_or : ∀ φ₁ φ₂ : QuantFreeFormula n, eval (or φ₁ φ₂) = eval φ₁ ∪ eval φ₂
+  | tru, _ => by simp [or, eval]
+  | fals, fals => by simp [or, eval]
+  | fals, tru => by simp [or, eval]
+  | ite' _ _ _, tru => by simp [or, eval]
+  | fals, ite' _ _ _ => by simp [or, eval]
+  | ite' _ _ _, fals => by simp [or, eval]
+  | ite' p φ ψ, ite' q χ ω => by
+    rw [or]
+    ext x
+    by_cases h1 : rel p q <;> by_cases h2 : p.eval x = 0 <;> by_cases h3 : q.eval x = 0
+      <;> simp_all [eval, eval_or]
+
+def and : ∀ (_φ₁ _φ₂ : QuantFreeFormula n), QuantFreeFormula n
+  | fals, _ => fals
+  | _, fals => fals
+  | tru, φ => φ
+  | φ, tru => φ
+  | ite' p φ ψ, ite' q χ ω =>
+    if rel p q
+    then ite' p (ite' q (φ.and χ) (φ.and ω)) (ite' q (ψ.and χ) (ψ.and ω))
+    else ite' q (ite' p (φ.and χ) (ψ.and χ)) (ite' p (φ.and ω) (ψ.and ω))
+
+@[simp]
+theorem eval_and : ∀ φ₁ φ₂ : QuantFreeFormula n, eval (and φ₁ φ₂) = eval φ₁ ∩ eval φ₂
+  | fals, _ => by simp [and, eval]
+  | tru, tru => by simp [and, eval]
+  | tru, fals => by simp [and, eval]
+  | ite' _ _ _, tru => by simp [and, eval]
+  | tru, ite' _ _ _ => by simp [and, eval]
+  | ite' _ _ _, fals => by simp [and, eval]
+  | ite' p φ ψ, ite' q χ ω => by
+    rw [and]
+    ext x
+    by_cases h1 : rel p q <;> by_cases h2 : p.eval x = 0 <;> by_cases h3 : q.eval x = 0
+      <;> simp_all [eval, eval_and]
 
 def iOrs {α : Type*} (l : List α) (f : α → QuantFreeFormula n) : QuantFreeFormula n :=
-  l.foldr (fun a φ => (f a).or φ) false
+  l.foldr (fun a φ => (f a).or φ) fals
 
 @[simp]
 theorem eval_ors  {α : Type*} (l : List α) (f : α → QuantFreeFormula n) :
@@ -50,34 +95,29 @@ theorem eval_ors  {α : Type*} (l : List α) (f : α → QuantFreeFormula n) :
     simp [iOrs, eval, ih, Set.ext_iff] at *
     simp [ih]
 
-def ands {α : Type*} (l : List α) (f : α → QuantFreeFormula n) : QuantFreeFormula n :=
-  l.foldr (fun a φ => (f a).and φ) true
+def iAnds {α : Type*} (l : List α) (f : α → QuantFreeFormula n) : QuantFreeFormula n :=
+  l.foldr (fun a φ => (f a).and φ) tru
 
 @[simp]
-theorem eval_ands {α : Type*} (l : List α) (f : α → QuantFreeFormula n) :
-    (ands l f).eval = ⋂ (a ∈ l), (f a).eval := by
+theorem eval_iAnds {α : Type*} (l : List α) (f : α → QuantFreeFormula n) :
+    (iAnds l f).eval = ⋂ (a ∈ l), (f a).eval := by
   induction l with
-  | nil => simp [ands, eval]
+  | nil => simp [iAnds, eval]
   | cons a l ih =>
-    simp [ands, eval, ih, Set.ext_iff] at *
+    simp [iAnds, eval, ih, Set.ext_iff] at *
     simp [ih]
 
 open Poly
 
 instance decidableEvalZero (x : Fin 0 → ℂ) : ∀ (φ : QuantFreeFormula 0), Decidable (x ∈ φ.eval)
-  | true => isTrue trivial
-  | false => isFalse not_false
-  | neZero p => decidable_of_iff (toInt p ≠ 0)
-      (by rcases p with ⟨⟨_⟩, _⟩; simp[Poly.eval, toInt])
-  | eqZero p => decidable_of_iff (toInt p = 0)
-      (by rcases p with ⟨⟨_⟩, _⟩; simp[Poly.eval, toInt])
-  | and φ ψ => by
-    have := decidableEvalZero x φ
-    have := decidableEvalZero x ψ
-    simp [eval]; infer_instance
-  | or φ ψ =>  by
-    have := decidableEvalZero x φ
-    have := decidableEvalZero x ψ
-    simp [eval]; infer_instance
+  | tru => isTrue trivial
+  | fals => isFalse not_false
+  | ite' p φ ψ =>
+      have := decidableEvalZero x φ
+      have := decidableEvalZero x ψ
+      decidable_of_iff ((if toInt p = 0 then x ∈ φ.eval else x ∈ ψ.eval) = true)
+        (by
+          rcases p with ⟨⟨_⟩, _⟩
+          split_ifs <;> simp[Poly.eval, toInt, *] <;> tauto)
 
 end QuantFreeFormula
